Ordered_Resolution_Prover/AFP_IsaFoR/AFP_Term.thy
@@ -1,0 +1,106 @@
+theory AFP_Term imports Main begin
+
+datatype (funs_term : 'f, vars_term : 'v) "term" =
+  is_Var: Var (the_Var: 'v) |
+  Fun 'f (args : "('f, 'v) term list")
+where
+  "args (Var _) = []"
+
+text \<open>
+  Reorient equations of the form @{term "Var x = t"} and @{term "Fun f ss = t"} to facilitate
+  simplification.
+\<close>
+setup \<open>
+  Reorient_Proc.add
+    (fn Const (@{const_name Var}, _) $ _ => true | _ => false)
+  #> Reorient_Proc.add
+    (fn Const (@{const_name Fun}, _) $ _ $ _ => true | _ => false)
+\<close>
+
+simproc_setup reorient_Var ("Var x = t") = Reorient_Proc.proc
+simproc_setup reorient_Fun ("Fun f ss = t") = Reorient_Proc.proc
+
+lemma finite_vars_term [simp]:
+  "finite (vars_term t)"
+  by (induct t) simp_all
+
+lemma finite_Union_vars_term:
+  "finite (\<Union>t \<in> set ts. vars_term t)"
+  by auto
+
+text \<open>
+  A \emph{substitution} is a mapping~$\sigma$ from variables to terms. We call a substitution that
+  alters the type of variables a \emph{general substitution}, since it does not have all properties
+  that are expected of (standard) substitutions (e.g., there is no empty substitution).
+\<close>
+type_synonym ('f, 'v, 'w) gsubst = "'v \<Rightarrow> ('f, 'w) term"
+type_synonym ('f, 'v) subst  = "('f, 'v, 'v) gsubst"
+
+fun subst_apply_term :: "('f, 'v) term \<Rightarrow> ('f, 'v, 'w) gsubst \<Rightarrow> ('f, 'w) term" (infixl "\<cdot>" 67)
+where
+  "Var x \<cdot> \<sigma> = \<sigma> x" |
+  "Fun f ss \<cdot> \<sigma> = Fun f (map (\<lambda>t. t \<cdot> \<sigma>) ss)"
+
+definition
+  subst_compose :: "('f, 'u, 'v) gsubst \<Rightarrow> ('f, 'v, 'w) gsubst \<Rightarrow> ('f, 'u, 'w) gsubst"
+  (infixl "\<circ>\<^sub>s" 75)
+where
+  "\<sigma> \<circ>\<^sub>s \<tau> = (\<lambda>x. (\<sigma> x) \<cdot> \<tau>)"
+
+lemma subst_subst_compose [simp]:
+  "t \<cdot> (\<sigma> \<circ>\<^sub>s \<tau>) = t \<cdot> \<sigma> \<cdot> \<tau>"
+by (induct t \<sigma> rule: subst_apply_term.induct) (simp add: subst_compose_def)+
+
+lemma subst_compose_assoc:
+  "\<sigma> \<circ>\<^sub>s \<tau> \<circ>\<^sub>s \<mu> = \<sigma> \<circ>\<^sub>s (\<tau> \<circ>\<^sub>s \<mu>)"
+proof (rule ext)
+  fix x show "(\<sigma> \<circ>\<^sub>s \<tau> \<circ>\<^sub>s \<mu>) x = (\<sigma> \<circ>\<^sub>s (\<tau> \<circ>\<^sub>s \<mu>)) x"
+  proof -
+    have "(\<sigma> \<circ>\<^sub>s \<tau> \<circ>\<^sub>s \<mu>) x = \<sigma>(x) \<cdot> \<tau> \<cdot> \<mu>" by (simp add: subst_compose_def)
+    also have "\<dots> = \<sigma>(x) \<cdot> (\<tau> \<circ>\<^sub>s \<mu>)" by simp
+    finally show ?thesis by (simp add: subst_compose_def)
+  qed
+qed
+
+lemma subst_apply_term_empty [simp]:
+  "t \<cdot> Var = t"
+proof (induct t)
+  case (Fun f ts)
+  from map_ext [rule_format, of ts _ id, OF Fun] show ?case by simp
+qed simp
+
+interpretation subst_monoid_mult: monoid_mult "Var" "op \<circ>\<^sub>s"
+  by (unfold_locales)
+     (simp add: subst_compose_assoc, simp_all add: subst_compose_def)
+
+lemma term_subst_eq:
+  assumes "\<And>x. x \<in> vars_term t \<Longrightarrow> \<sigma> x = \<tau> x"
+  shows "t \<cdot> \<sigma> = t \<cdot> \<tau>"
+  using assms by (induct t) (auto)
+
+lemma term_subst_eq_rev:
+  "t \<cdot> \<sigma> = t \<cdot> \<tau> \<Longrightarrow> \<forall>x \<in> vars_term t. \<sigma> x = \<tau> x"
+proof (induct t)
+  case (Fun f ts)
+  thus ?case by auto
+qed simp
+
+lemma term_subst_eq_conv:
+  "(t \<cdot> \<sigma> = t \<cdot> \<tau>) = (\<forall>x \<in> vars_term t. \<sigma> x = \<tau> x)"
+  using term_subst_eq [of t \<sigma> \<tau>] term_subst_eq_rev [of t \<sigma> \<tau>] by auto
+
+lemma subst_term_eqI:
+  assumes "(\<And>t. t \<cdot> \<sigma> = t \<cdot> \<tau>)"
+  shows "\<sigma> = \<tau>"
+proof (rule ext)
+  fix x
+  show "\<sigma> x = \<tau> x" using assms [of "Var x"] by simp
+qed
+
+definition subst_domain :: "('f, 'v) subst \<Rightarrow> 'v set" where
+  "subst_domain \<sigma> = {x. \<sigma> x \<noteq> Var x}"
+
+definition var_renaming :: "('f, 'v) subst \<Rightarrow> bool" where
+  "var_renaming \<sigma> \<longleftrightarrow> (\<forall>x. is_Var (\<sigma> x)) \<and> inj_on \<sigma> (subst_domain \<sigma>)"
+
+end
